Added some patches to SVN. Ouch, this is the point I really regret choosing SVN.

TermEquality.v
@@ -1,3 +1,4 @@
+Require Import Prelims.
 Require Import Signature.
 Require Import Variables.
 Require Import Term.
@@ -19,15 +20,29 @@ Notation terms := (vector term).
 CoInductive term_bis : term -> term -> Prop :=
   | Var_bis : forall x, term_bis (Var x) (Var x)
   | Fun_bis : forall f v w,
-              (forall i, term_bis (v i) (w i)) ->
+              (forall n (H : n < arity f), term_bis (Vnth v H) (Vnth w H)) ->
               term_bis (Fun f v) (Fun f w).
+
+(*
+CoInductive term_bis : term -> term -> Prop :=
+  | Var_bis : forall x, term_bis (Var x) (Var x)
+  | Fun_bis : forall f v w,
+              terms_bis v w ->
+              term_bis (Fun f v) (Fun f w)
+with terms_bis : forall n, terms n -> terms n -> Prop :=
+  | O_bis  : forall (v w : terms 0), terms_bis v w
+  | Sn_bis : forall n (v w : terms n) t s,
+             terms_bis v w ->
+             term_bis t s ->
+             terms_bis (Vcons t v) (Vcons s w).
+*)
 
 (* Equality of infinite terms up to a given depth *)
 Inductive term_eq_up_to : nat -> term -> term -> Prop :=
   | teut_0   : forall t u : term, term_eq_up_to 0 t u
   | teut_var : forall n x, term_eq_up_to n (Var x) (Var x)
   | teut_fun : forall n f v w,
-               (forall i, term_eq_up_to n (v i) (w i)) ->
+               (forall m (H : m < arity f), term_eq_up_to n (Vnth v H) (Vnth w H)) ->
                term_eq_up_to (S n) (Fun f v) (Fun f w).
 
 Definition term_eq (t u : term) :=
@@ -39,7 +54,7 @@ Definition term_eq (t u : term) :=
 Lemma teut_fun_inv :
   forall n f v w,
   term_eq_up_to (S n) (Fun f v) (Fun f w) ->
-  forall i, term_eq_up_to n (v i) (w i).
+  forall m (H : m < arity f), term_eq_up_to n (Vnth v H) (Vnth w H).
 Proof.
 intros n f v w H.
 dependent destruction H.
@@ -49,9 +64,9 @@ Qed.
 Lemma term_eq_fun_inv :
   forall f v w,
   term_eq (Fun f v) (Fun f w) ->
-  forall i, term_eq (v i) (w i).
+  forall n (H : n < arity f), term_eq (Vnth v H) (Vnth w H).
 Proof.
-intros f v w H i n.
+intros f v w H m h n.
 apply teut_fun_inv with (1 := H (S n)).
 Qed.
 
@@ -65,8 +80,8 @@ constructor.
 destruct H.
 constructor.
 constructor.
-intro i.
-apply IHn with (1:=(H i)).
+intros m h.
+apply IHn with (1:=(H m h)).
 Qed.
 
 Lemma term_eq_fun_inv_symbol :
@@ -90,7 +105,7 @@ assert (H0 := H 1); inversion_clear H0.
 assert (H0 := term_eq_fun_inv_symbol H).
 dependent destruction H0.
 apply Fun_bis.
-intro i.
+intros n h.
 assert (H0 := term_eq_fun_inv H).
 apply eq2bis.
 apply H0.
@@ -109,8 +124,8 @@ inversion_clear H1; intro H2.
 assumption.
 dependent destruction H2.
 constructor.
-intro i.
-apply IH with (u := w i); trivial.
+intros m h.
+apply IH with (u := Vnth w h); trivial.
 Qed.
 
 (* TODO: define term_eq_refl and term_eq_symm using the
@@ -137,7 +152,7 @@ constructor.
 destruct t.
 constructor.
 constructor.
-intro.
+intros.
 apply IH.
 Qed.
 
@@ -151,7 +166,7 @@ constructor.
 inversion_clear H'.
 constructor.
 constructor.
-intro.
+intros.
 apply IHn.
 apply H.
 Qed.
@@ -165,14 +180,14 @@ Qed.
 Lemma term_bis_refl : forall t, term_bis t t.
 cofix.
 destruct t as [x|f v]; constructor.
-intro i.
+intros n h.
 apply term_bis_refl.
 Qed.
 
 Lemma term_bis_symm : forall t u, term_bis t u -> term_bis u t.
 cofix.
 destruct 1 as [x|f v w H]; constructor.
-intro i.
+intros n h.
 apply term_bis_symm.
 apply H.
 Qed.
@@ -188,8 +203,8 @@ inversion H2 as [|g ys' zs].
 *)
 dependent destruction H2.
 rename w into zs, H into H2.
-constructor; intro i.
-apply term_bis_trans with (1:=(H1 i)) (2:=(H2 i)).
+constructor; intros n h.
+apply term_bis_trans with (1:=(H1 n h)) (2:=(H2 n h)).
 Qed.
 
 End TermEquality.
