ContextEquality.v
@@ -1,3 +1,4 @@
+Require Import Prelims.
 Require Import Signature.
 Require Import Variables.
 Require Import Context.
@@ -26,9 +27,9 @@ Notation context := (context F X).
 Inductive context_bis : context -> context -> Prop :=
   | Hole_bis : context_bis Hole Hole
   | CFun_bis : forall f i j H (v v' : terms i) c c' (w w' : terms j),
-               (forall i, term_bis (v i) (v' i)) ->
+               (forall n (H : n < i), term_bis (Vnth v H) (Vnth v' H)) ->
                context_bis c c' ->
-               (forall i, term_bis (w i) (w' i)) ->
+               (forall n (H : n < j), term_bis (Vnth w H) (Vnth w' H)) ->
                context_bis (CFun f H v c w) (CFun f H v' c' w').
 
 (* Equality of contexts up to a given depth *)
@@ -36,9 +37,9 @@ Inductive context_eq_up_to : nat -> context -> context -> Prop :=
   | ceut_0    : forall c c' : context, context_eq_up_to 0 c c'
   | ceut_hole : forall n, context_eq_up_to n Hole Hole
   | ceut_cfun : forall n f i j H (v v' : terms i) c c' (w w' : terms j),
-                (forall i, term_eq_up_to n (v i) (v' i)) ->
+                (forall n (H : n < i), term_eq_up_to n (Vnth v H) (Vnth v' H)) ->
                 context_eq_up_to n c c' ->
-                (forall i, term_eq_up_to n (w i) (w' i)) ->
+                (forall n (H : n < j), term_eq_up_to n (Vnth w H) (Vnth w' H)) ->
                 context_eq_up_to (S n) (CFun f H v c w) (CFun f H v' c' w').
 
 Definition context_eq (c c' : context) :=
