FiniteTerm.v
@@ -1,9 +1,13 @@
+Require Import Prelims.
 Require Import Max. (* TODO: deprecated in Coq 8.3? Max.v -> Peano.v *)
 Require Import List.
 Require Export Signature.
 Require Export Variables.
-Require Export Vector.
+Require Export Bvector.
 
+
+Implicit Arguments Vnil [A].
+Implicit Arguments Vcons [A n].
 
 Set Implicit Arguments.
 
@@ -18,8 +22,39 @@ Inductive finite_term : Type :=
   | FVar : X -> finite_term
   | FFun : forall f : F, vector finite_term (arity f) -> finite_term.
 
+Reset finite_term_rect.
+
 Notation fterm := (finite_term).
 Notation fterms := (vector fterm).
+
+Section InductionPrinciple.
+
+Variables
+  (P : fterm -> Type)
+  (Q : forall n, fterms n -> Type).
+
+Hypotheses
+  (H1 : forall x, P (FVar x))
+  (H2 : forall f v, Q v -> P (FFun f v))
+  (H3 : Q Vnil)
+  (H4 : forall t n (v : fterms n), P t -> Q v -> Q (Vcons t v)).
+
+Fixpoint finite_term_rect t : P t :=
+  match t as t return P t with
+    | FVar x => H1 x
+    | FFun f v =>
+      let fix finite_terms_rect n (v : fterms n) {struct v} : Q v :=
+        match v as v return Q v with
+          | Vnil => H3
+          | Vcons t' n' v' => H4 (finite_term_rect t') (finite_terms_rect n' v')
+        end
+    in H2 f (finite_terms_rect (arity f) v)
+  end.
+
+End InductionPrinciple.
+
+Definition finite_term_ind (P : fterm -> Prop) (Q : forall n, fterms n -> Prop) :=
+  finite_term_rect P Q.
 
 (* TODO: Bool or prop? *)
 Definition is_var (t : fterm) : bool :=
@@ -31,21 +66,21 @@ Definition is_var (t : fterm) : bool :=
 Fixpoint size (t : fterm) : nat :=
   match t with
   | FVar _      => 1
-  | FFun _ args => 1 + vfold 0 plus (vmap size args)
+  | FFun _ args => 1 + Vfold_right plus (Vmap size args) 0
                     (* vfold 0 (plus * size) args *)
   end.
 
 Fixpoint pattern_depth (t : fterm) : nat :=
   match t with
   | FVar _      => 0
-  | FFun _ args => 1 + vfold 0 max (vmap pattern_depth args)
+  | FFun _ args => 1 + Vfold_right max (Vmap pattern_depth args) 0
   end.
 
 (* List of variable occurrences in a finite term *)
 Fixpoint vars (t : fterm) : list X :=
   match t with
   | FVar x      => x :: nil
-  | FFun _ args => vfold nil (@app X) (vmap vars args)
+  | FFun _ args => Vfold_right (@app X) (Vmap vars args) nil
   end.
 
 (* A finite term is linear if it has no duplicate variable occurrences *)
