RewritingOrdinalSequence.v
@@ -1,6 +1,5 @@
 (* Inductive defintion for rewriting sequences *)
 
-
 Require Import Prelims.
 Require Export List.
 Require Export FiniteTerm.
@@ -10,6 +9,9 @@ Require Export Context.
 Require Export PreOrdinal.
 Require Export TermEquality.
 
+
+Implicit Arguments inl [A].
+Implicit Arguments inr [B].
 
 Set Implicit Arguments.
 
