Vector2.v
@@ -2,6 +2,9 @@ Require Import Prelims.
 Require Import Equality.
 
 
+Implicit Arguments inl [A].
+Implicit Arguments inr [B].
+
 Set Implicit Arguments.
 
 
